Uppaal_Networks/AbsInt/State_Smart.thy
@@ -4,17 +4,17 @@ begin
 
 type_synonym 'a arstate = "'a list toption"
 
-datatype 'a smart_base = Smart "'a arstate" power_bool
-type_synonym 'a smart = "'a smart_base option"
+datatype ('a, 'b) smart_base = Smart 'b "'a arstate" power_bool
+type_synonym ('a, 'b) smart = "('a, 'b) smart_base option"
 
-instantiation smart_base :: (absword) order_top
+instantiation smart_base :: (absword, absstack) order_top
 begin
-  definition[simp]: "\<top> \<equiv> Smart \<top> \<top>"
+  definition[simp]: "\<top> \<equiv> Smart \<top> \<top> \<top>"
 
-  fun less_eq_smart_base :: "'a smart_base \<Rightarrow> 'a smart_base \<Rightarrow> bool" where
-    "less_eq_smart_base (Smart aregs aflag) (Smart bregs bflag) \<longleftrightarrow> aregs \<le> bregs \<and> aflag \<le> bflag"
+  fun less_eq_smart_base :: "('a, 'b) smart_base \<Rightarrow> ('a, 'b) smart_base \<Rightarrow> bool" where
+    "less_eq_smart_base (Smart astack aregs aflag) (Smart bstack bregs bflag) \<longleftrightarrow> astack \<le> bstack \<and> aregs \<le> bregs \<and> aflag \<le> bflag"
 
-  fun less_smart_base :: "'a smart_base \<Rightarrow> 'a smart_base \<Rightarrow> bool" where
+  fun less_smart_base :: "('a, 'b) smart_base \<Rightarrow> ('a, 'b) smart_base \<Rightarrow> bool" where
     "less_smart_base a b \<longleftrightarrow> a \<le> b \<and> \<not> b \<le> a"
 instance
 proof (standard, goal_cases)
@@ -29,11 +29,11 @@ next
 qed simp
 end
 
-instantiation smart_base :: (absword) semilattice_sup
+instantiation smart_base :: (absword, absstack) semilattice_sup
 begin
-  fun sup_smart_base :: "'a smart_base \<Rightarrow> 'a smart_base \<Rightarrow> 'a smart_base" where
-    "sup_smart_base (Smart aregs aflag) (Smart bregs bflag) =
-      Smart (aregs \<squnion> bregs) (aflag \<squnion> bflag)"
+  fun sup_smart_base :: "('a, 'b) smart_base \<Rightarrow> ('a, 'b) smart_base \<Rightarrow> ('a, 'b) smart_base" where
+    "sup_smart_base (Smart astack aregs aflag) (Smart bstack bregs bflag) =
+      Smart (astack \<squnion> bstack) (aregs \<squnion> bregs) (aflag \<squnion> bflag)"
 instance
 proof (standard, goal_cases)
   case (1 x y) show ?case by (cases x; cases y; simp)
@@ -85,20 +85,32 @@ qed
 
 lemma mono_gamma_power_bool: "a \<le> b \<Longrightarrow> \<gamma>_power_bool a \<le> \<gamma>_power_bool b" by (cases a; cases b; simp)
 
-fun \<gamma>_smart :: "'a smart \<Rightarrow> collect_state set" where
+fun \<gamma>_smart :: "('a, 'b) smart \<Rightarrow> collect_state set" where
   "\<gamma>_smart None = \<bottom>" |
-  "\<gamma>_smart (Some (Smart aregs aflag)) = {(stack, rstate, flag, nl). rstate \<in> \<gamma>_regs aregs \<and> flag \<in> \<gamma>_power_bool aflag}"
+  "\<gamma>_smart (Some (Smart astack aregs aflag)) = {(stack, rstate, flag, nl). stack \<in> \<gamma>_stack astack \<and> rstate \<in> \<gamma>_regs aregs \<and> flag \<in> \<gamma>_power_bool aflag}"
 
-fun step_smart_base :: "instr \<Rightarrow> addr \<Rightarrow> 'a smart_base \<Rightarrow> 'a smart state_map" where
-  "step_smart_base (JMPZ target) pc (Smart regs BTrue)  = single (Suc pc) (Some (Smart regs BTrue))" |
-  "step_smart_base (JMPZ target) pc (Smart regs BFalse) = single target (Some (Smart regs BFalse))" |
-  "step_smart_base (JMPZ target) pc (Smart regs BBoth)  = deep_merge {(target, Some (Smart regs BBoth)), (Suc pc, Some (Smart regs BBoth))}" |
-  "step_smart_base ADD           pc (Smart regs flag)   = single (Suc pc) (Some (Smart regs flag))" |
-  "step_smart_base NOT           pc (Smart regs flag)   = single (Suc pc) (Some (Smart regs (not flag)))" |
-  "step_smart_base AND           pc (Smart regs flag)   = single (Suc pc) (Some (Smart regs BBoth))" |
+fun step_smart_base :: "instr \<Rightarrow> addr \<Rightarrow> ('a::absword, 'b::absstack) smart_base \<Rightarrow> ('a, 'b) smart state_map" where
+  "step_smart_base (JMPZ target) pc (Smart stack regs BTrue)  = single (Suc pc) (Some (Smart stack regs BTrue))" |
+  "step_smart_base (JMPZ target) pc (Smart stack regs BFalse) = single target (Some (Smart stack regs BFalse))" |
+  "step_smart_base (JMPZ target) pc (Smart stack regs BBoth)  = deep_merge {(target, Some (Smart stack regs BBoth)), (Suc pc, Some (Smart stack regs BBoth))}" |
+
+  "step_smart_base ADD           pc (Smart stack regs flag)   =
+    (let (bstack, b) = pop stack;
+        (astack, a) = pop bstack;
+        rstack = push astack (aplus a b) in
+    single (Suc pc) (Some (Smart rstack regs flag)))" |
+
+  "step_smart_base NOT           pc (Smart stack regs flag)   = single (Suc pc) (Some (Smart (fst (pop stack)) regs (not flag)))" |
+
+  "step_smart_base AND           pc (Smart stack regs flag)   =
+    (let (rstack, a) = pop stack;
+         r0 = if contains a 0 then {Some (Smart (fst (pop stack)) regs (and BFalse flag))} else {};
+         r1 = r0 \<union> (if contains a 1 then {Some (Smart (fst (pop stack)) regs (and BTrue flag))} else {})
+     in deep_merge ((\<lambda>v. (Suc pc, v)) ` r1))" |
+
   "step_smart_base _ _ _ = \<top>"
 
-fun step_smart :: "('a::absword) smart astep" where
+fun step_smart :: "('a::absword, 'b::absstack) smart astep" where
   "step_smart _ _ None = \<bottom>" |
   "step_smart op pc (Some a) = step_smart_base op pc a"
 
@@ -107,13 +119,15 @@ lemma gamma_smart_mono:
   shows "\<gamma>_smart a \<subseteq> \<gamma>_smart b"
 proof (intro Set.subsetI)
   fix x assume ass: "x \<in> \<gamma>_smart a"
-  from ass obtain aregs aflag where asplit: "a = Some (Smart aregs aflag)" by (metis \<gamma>_smart.elims empty_iff)
-  from this assms obtain bregs bflag where bsplit: "b = Some (Smart bregs bflag)" by (metis \<gamma>_smart.cases less_eq_option.simps(2))
+  from ass obtain astack aregs aflag where asplit: "a = Some (Smart astack aregs aflag)" by (metis \<gamma>_smart.elims empty_iff)
+  from this assms obtain bstack bregs bflag where bsplit: "b = Some (Smart bstack bregs bflag)" by (metis \<gamma>_smart.cases less_eq_option.simps(2))
   from ass obtain stack rstate flag nl where xsplit: "x = (stack, rstate, flag, nl)" using prod_cases4 by blast 
-  from assms asplit bsplit have fine_le: "aregs \<le> bregs" "aflag \<le> bflag" by auto
-  from asplit xsplit ass have "rstate \<in> \<gamma>_regs aregs \<and> flag \<in> \<gamma>_power_bool aflag" by simp
-  from this fine_le have "rstate \<in> \<gamma>_regs bregs" "flag \<in> \<gamma>_power_bool bflag" using mono_gamma_power_bool mono_gamma_regs by (blast, blast)
-  from this bsplit xsplit show "x \<in> \<gamma>_smart b" by simp
+  from assms asplit bsplit have fine_le: "astack \<le> bstack" "aregs \<le> bregs" "aflag \<le> bflag" by auto
+  from asplit xsplit ass have ain: "stack \<in> \<gamma>_stack astack \<and> rstate \<in> \<gamma>_regs aregs \<and> flag \<in> \<gamma>_power_bool aflag" by simp
+  from ain fine_le have regs: "rstate \<in> \<gamma>_regs bregs" using mono_gamma_regs by blast
+  from ain fine_le have flag: "flag \<in> \<gamma>_power_bool bflag" using mono_gamma_power_bool by blast
+  from ain fine_le have stack: "stack \<in> \<gamma>_stack bstack" using mono_gamma_stack by blast
+  from regs flag stack bsplit xsplit show "x \<in> \<gamma>_smart b" by simp
 qed
 
 lemma gamma_smart_top: "\<gamma>_smart \<top> = \<top>"
@@ -123,12 +137,12 @@ proof -
 qed
 
 lemma step_smart_nonbot_correct:
-  assumes "ost \<in> lookup (collect_step op ipc (\<gamma>_smart (Some (Smart iaregs iaflag)))) opc"
-  shows "ost \<in> \<gamma>_smart (lookup (step_smart op ipc (Some (Smart iaregs iaflag))) opc)"
+  assumes "ost \<in> lookup (collect_step op ipc (\<gamma>_smart (Some (Smart iastack iaregs iaflag)))) opc"
+  shows "ost \<in> \<gamma>_smart (lookup (step_smart op ipc (Some (Smart iastack iaregs iaflag))) opc)"
 proof -
   obtain ocstack ocregs ocflag ocrs where ost_split: "ost = (ocstack, ocregs, ocflag, ocrs)" by (rule prod_cases4)
 
-  let ?ists = "\<gamma>_smart (Some (Smart iaregs iaflag))"
+  let ?ists = "\<gamma>_smart (Some (Smart iastack iaregs iaflag))"
   from assms have "\<exists>ist\<in>?ists. step op (ipc, ist) = Some (opc, ost)" by simp
   from this obtain ist where ist_step: "ist \<in> ?ists" "step op (ipc, ist) = Some (opc, ost)" ..
   obtain icstack icregs icflag icrs where ist_split: "ist = (icstack, icregs, icflag, icrs)" by (rule prod_cases4)
@@ -137,8 +151,7 @@ proof -
     "(icstack, icregs, icflag, icrs) \<in> ?ists"
     "step op (ipc, (icstack, icregs, icflag, icrs)) = Some (opc, (ocstack, ocregs, ocflag, ocrs))" by auto
 
-  (* more properties can be added here if \<gamma>_smart gets updated *)
-  from ist_step(1) ist_split have ist_props: "icregs \<in> \<gamma>_regs iaregs" "icflag \<in> \<gamma>_power_bool iaflag" by auto
+  from ist_step(1) ist_split have ist_props: "icstack \<in> \<gamma>_stack iastack" "icregs \<in> \<gamma>_regs iaregs" "icflag \<in> \<gamma>_power_bool iaflag" by auto
 
   show ?thesis 
   proof (cases op)
@@ -152,55 +165,64 @@ proof -
       case BTrue
       from this have "icflag = True" using ist_props by simp
       from this JMPZ ist_split_step(2) have "opc = Suc ipc" using step_jmpz_true(4) by blast
-      from this BTrue JMPZ have "lookup (step_smart op ipc (Some (Smart iaregs iaflag))) opc = Some (Smart iaregs iaflag)" using single_lookup by simp
-      then show ?thesis using ist_split flag_preserve ist_step(1) ost_split regs_preserve by simp
+      from this BTrue JMPZ have "lookup (step_smart op ipc (Some (Smart iastack iaregs iaflag))) opc = Some (Smart iastack iaregs iaflag)" using single_lookup by simp
+      then show ?thesis using ist_split flag_preserve ist_step(1) ost_split regs_preserve stack_preserve by simp
     next
       case BFalse
       from this have "icflag = False" using ist_props by simp
       from this JMPZ ist_split_step(2) have "opc = target" using step_jmpz_false(4) by blast
-      from this BFalse JMPZ have "lookup (step_smart op ipc (Some (Smart iaregs iaflag))) opc = Some (Smart iaregs iaflag)" using single_lookup by simp
-      then show ?thesis using ist_split flag_preserve ist_step(1) ost_split regs_preserve by simp
+      from this BFalse JMPZ have "lookup (step_smart op ipc (Some (Smart iastack iaregs iaflag))) opc = Some (Smart iastack iaregs iaflag)" using single_lookup by simp
+      then show ?thesis using ist_split flag_preserve ist_step(1) ost_split regs_preserve stack_preserve by simp
     next
       case BBoth
       then show ?thesis
       proof (cases icflag)
         case True
         from this JMPZ ist_split_step(2) have "opc = Suc ipc" using step_jmpz_true(4) by (metis(full_types))
-        from this BBoth JMPZ have lookup: "Some (Smart iaregs iaflag) \<le> lookup (step_smart op ipc (Some (Smart iaregs iaflag))) opc" using deep_merge_lookup
+        from this BBoth JMPZ have lookup: "Some (Smart iastack iaregs iaflag) \<le> lookup (step_smart op ipc (Some (Smart iastack iaregs iaflag))) opc" using deep_merge_lookup
           by (metis insert_iff step_smart.simps(2) step_smart_base.simps(3))
-        have "ost \<in> \<gamma>_smart (Some (Smart iaregs iaflag))" using ist_split flag_preserve ist_step(1) ost_split regs_preserve by simp
+        have "ost \<in> \<gamma>_smart (Some (Smart iastack iaregs iaflag))" using ist_split flag_preserve ist_step(1) ost_split regs_preserve stack_preserve by simp
         from this lookup show ?thesis using gamma_smart_mono by blast
       next
         case False
         from this JMPZ ist_split_step(2) have "opc = target" using step_jmpz_false(4) by (metis(full_types))
-        from this BBoth JMPZ have lookup: "Some (Smart iaregs iaflag) \<le> lookup (step_smart op ipc (Some (Smart iaregs iaflag))) opc" using deep_merge_lookup
+        from this BBoth JMPZ have lookup: "Some (Smart iastack iaregs iaflag) \<le> lookup (step_smart op ipc (Some (Smart iastack iaregs iaflag))) opc" using deep_merge_lookup
           by (metis insert_iff step_smart.simps(2) step_smart_base.simps(3))
-        have "ost \<in> \<gamma>_smart (Some (Smart iaregs iaflag))" using ist_split flag_preserve ist_step(1) ost_split regs_preserve by simp
+        have "ost \<in> \<gamma>_smart (Some (Smart iastack iaregs iaflag))" using ist_split flag_preserve ist_step(1) ost_split regs_preserve stack_preserve by simp
         from this lookup show ?thesis using gamma_smart_mono by blast
       qed
     qed
   next
     case ADD
-    hence f1: "step ADD (ipc, icstack, icregs, icflag, icrs) = Some (opc, ocstack, ocregs, ocflag, ocrs)"
-      using ist_split_step(2) by presburger
+    hence f1: "step ADD (ipc, icstack, icregs, icflag, icrs) = Some (opc, ocstack, ocregs, ocflag, ocrs)" using ist_split_step(2) by simp
     then have f2: "ocregs = icregs" by (simp add: step_add(2))
-    have "ocflag = icflag" using f1 by (simp add: step_add(3))
-    then show ?thesis using f2 f1 ADD ist_split_step(1) ost_split step_add(1) by force
+    have flag: "ocflag = icflag" using f1 by (simp add: step_add(3))
+    from f1 obtain a b rest where stack: "icstack = a # b # rest" "ocstack = (a + b) # rest" using step_add(5) by blast
+    let ?oastack = "let (bstack, b) = pop iastack;
+        (astack, a) = pop bstack in
+        push astack (aplus a b)"
+    have lookup: "lookup (step_smart op ipc (Some (Smart iastack iaregs iaflag))) opc = (Some (Smart ?oastack iaregs iaflag))"
+      by (metis (mono_tags, lifting) ADD case_prod_beta' f1 single_lookup step_add(1) step_smart.simps(2) step_smart_base.simps(4))
+    have "ocstack \<in> \<gamma>_stack ?oastack"
+      by (smt case_prod_beta' ist_props(1) plus_correct pop_return_correct pop_stack_correct push_correct stack(1) stack(2))
+    then show ?thesis using f2 flag ist_props(2) ist_props(3) lookup ost_split by auto
   next
     case NOT
     from NOT ist_split_step have pc: "opc = Suc ipc" using step_not(1) by blast
     from NOT ist_split_step have regs_preserve: "ocregs = icregs" using step_not(2) by blast
     from NOT ist_split_step have flag: "ocflag = (\<not> icflag)" using step_not(3) by blast
     from NOT ist_split_step have rs_preserve: "ocrs = icrs" using step_not(4) by blast
-    then show ?thesis using NOT flag ist_props(1) ist_props(2) ost_split regs_preserve pc by (cases iaflag, auto)
+    from NOT ist_split_step obtain ia where pop: "icstack = ia # ocstack" using step_not(5) by blast
+    from this have stack: "ocstack \<in> \<gamma>_stack (fst (pop iastack))" using pop_stack_correct ist_props(1) by simp
+    have regs: "ocregs \<in> \<gamma>_regs iaregs" by (simp add: ist_props(2) regs_preserve)
+    have flag: "ocflag \<in> \<gamma>_power_bool (not iaflag)" using power_bool_not by (simp add: flag ist_props(3)) 
+    from stack regs flag pc show ?thesis by (simp add: NOT ost_split)
   next
     case AND
-    have f1: "step AND (ipc, icstack, icregs, icflag, icrs) = Some (opc, ocstack, ocregs, ocflag, ocrs)"
-      using AND ist_split_step(2) by blast
-    then have "ocregs = icregs"
-      by (simp add: step_and(2))
-    then show ?thesis
-      using f1 AND ist_split_step(1) ost_split step_and(1) by auto
+    have f1: "step AND (ipc, icstack, icregs, icflag, icrs) = Some (opc, ocstack, ocregs, ocflag, ocrs)" using AND ist_split_step(2) by blast
+    then have "ocregs = icregs" by (simp add: step_and(2))
+    from f1 obtain ia where "icstack = ia # ocstack" "ia = 1 \<or> ia = 0" "ocflag = (ia = 1 \<and> icflag)" using step_and(4) by blast
+    then show ?thesis using f1 AND ist_split_step(1) ost_split step_and(1) sorry
   next
     case LT
     then show ?thesis by auto
@@ -264,8 +286,8 @@ next
     then show ?thesis by simp
   next
     case False
-    have "lookup (collect_step op ipc (\<gamma>_smart (Some (Smart regs flag)))) pc
-          \<le> \<gamma>_smart (lookup (step_smart op ipc (Some (Smart regs flag))) pc)" for regs flag
+    have "lookup (collect_step op ipc (\<gamma>_smart (Some (Smart stack regs flag)))) pc
+          \<le> \<gamma>_smart (lookup (step_smart op ipc (Some (Smart stack regs flag))) pc)" for stack regs flag
       using step_smart_nonbot_correct by blast
     from this False show ?thesis by (metis \<gamma>_smart.elims bot_option_def)
   qed
