Uppaal_Networks/AbsInt/Stack.thy
@@ -2,13 +2,13 @@ theory Stack
   imports Word ListLattice
 begin
 
-class astack = bounded_semilattice_sup_bot + order_top
+class absstack = bounded_semilattice_sup_bot + order_top
 
 locale AbsStack = AbsWord +
-  fixes \<gamma>_stack :: "('b::astack) \<Rightarrow> stack set" and
+  fixes \<gamma>_stack :: "('b::absstack) \<Rightarrow> stack set" and
         push :: "'b \<Rightarrow> ('a::absword) \<Rightarrow> 'b" and
         pop :: "'b \<Rightarrow> ('b * 'a)"
-  assumes stack_mono_gamma: "a \<le> b \<Longrightarrow> \<gamma>_stack a \<le> \<gamma>_stack b"
+  assumes mono_gamma_stack: "a \<le> b \<Longrightarrow> \<gamma>_stack a \<le> \<gamma>_stack b"
   and gamma_Top[simp]: "\<gamma>_stack \<top> = \<top>"
   and push_correct: "c \<in> \<gamma>_stack b \<Longrightarrow> cx \<in> \<gamma>_word x \<Longrightarrow> (cx # c) \<in> \<gamma>_stack (push b x)"
   and pop_stack_correct:  "(cx # c) \<in> \<gamma>_stack b \<Longrightarrow> c \<in> \<gamma>_stack (fst (pop b))"
