Uppaal_Networks/AbsInt/Word.thy
@@ -1,5 +1,5 @@
 theory Word
-  imports AbsInt
+  imports AbsInt PowerBool
 begin
 
 section \<open>Abstraction of Machine Words\<close>
@@ -9,7 +9,11 @@ class absword = bounded_semilattice_sup_bot + order_top
 
 locale AbsWord =
 fixes \<gamma>_word :: "('a::absword) \<Rightarrow> int set"
-  assumes mono_gamma: "a \<le> b \<Longrightarrow> \<gamma>_word a \<le> \<gamma>_word b"
+  and aplus :: "'a \<Rightarrow> 'a \<Rightarrow> 'a"
+  and contains :: "'a \<Rightarrow> int \<Rightarrow> bool"
+assumes mono_gamma: "a \<le> b \<Longrightarrow> \<gamma>_word a \<le> \<gamma>_word b"
   and gamma_Top[simp]: "\<gamma>_word \<top> = UNIV"
+  and plus_correct: "x \<in> \<gamma>_word a \<Longrightarrow> y \<in> \<gamma>_word b \<Longrightarrow> (x + y) \<in> \<gamma>_word (aplus a b)"
+  and contains_correct: "contains a x \<longleftrightarrow> x \<in> \<gamma>_word a"
 
 end
